Mt/Task/Impl.lean
@@ -26,9 +26,9 @@ def panic {T : Type} (msg : String) : TaskM spec T
 | r, s => IterationResult.Panic r s msg
 
 def atomic_assert
-  (cond : spec.Reservation -> spec.State -> Bool)
+  (cond : spec.State -> Bool)
   : TaskM spec Unit
-| r, s =>if cond r s then
+| r, s => if cond s then
     IterationResult.Done r s ⟨⟩
   else
     IterationResult.Panic r s "Assertion failed"
