Mt/Task/Validation.lean
@@ -57,4 +57,56 @@ theorem valid_bind {U V : Type}
       exact valid_bind motive_u mu_valid.right f_valid
 termination_by valid_bind => mu
 
+theorem valid_rmr {T : Type}
+  {f : spec.Reservation -> spec.State -> T × spec.Reservation × spec.State}
+  {r assuming motive}
+  (f_valid : ∀ env_r s,
+    assuming (env_r + r) →
+    spec.validate (env_r + r) s →
+    match f r s with
+    | ⟨t, r', s'⟩ => spec.validate (env_r + r') s' ∧ motive t r'
+  )
+  : (atomic_read_modify_read f).valid r assuming motive :=by
+  rw [valid]
+  intro env_r s assuming_true initial_valid
+  rw [iterate_rmr]
+  exact f_valid env_r s assuming_true initial_valid
+
+theorem valid_rm
+  {f : spec.Reservation -> spec.State -> spec.Reservation × spec.State}
+  {r assuming motive}
+  (f_valid : ∀ env_r s,
+    assuming (env_r + r) →
+    spec.validate (env_r + r) s →
+    match f r s with
+    | ⟨r', s'⟩ => spec.validate (env_r + r') s' ∧ motive ⟨⟩ r')
+  : (atomic_read_modify f).valid r assuming motive :=valid_rmr f_valid
+
+theorem valid_read
+  {f : spec.Reservation -> spec.State -> T × spec.Reservation}
+  {r assuming motive}
+  (f_valid : ∀ env_r s,
+    assuming (env_r + r) →
+    spec.validate (env_r + r) s →
+    match f r s with
+    | ⟨t, r'⟩ => spec.validate (env_r + r') s ∧ motive t r')
+  : (atomic_read f).valid r assuming motive :=valid_rmr f_valid
+
+theorem valid_assert
+  {cond : spec.State -> Bool}
+  {r assuming motive}
+  (motive_holds : motive ⟨⟩ r)
+  (assertion_succeeds : ∀ env_r s,
+    assuming (env_r + r) →
+    spec.validate (env_r + r) s →
+    cond s)
+  : (atomic_assert cond).valid r assuming motive :=by
+  rw [valid]
+  intro env_r s assuming_true initial_valid
+  rw [iterate_assert]
+  have cond_true :=assertion_succeeds env_r s assuming_true initial_valid
+  rw [cond_true]
+  simp only [ite_true]
+  exact ⟨initial_valid, motive_holds⟩
+
 end Mt.TaskM
